An attempt of fixing forward.v

floyd/forward.v
@@ -356,23 +356,6 @@ destruct (Map.get (ve_of rho) i) as [[? ?]|]; try contradiction.
 destruct H; subst; apply Coq.Init.Logic.I.
 Qed.
 
-Lemma gvar_isptr:
-  forall i v rho, locald_denote (gvar i v) rho -> isptr v.
-Proof.
-intros. hnf in H.
-destruct (Map.get (ve_of rho) i) as [[? ?]|]; try contradiction.
-destruct (Map.get (ge_of rho) i); try contradiction.
-subst; apply Coq.Init.Logic.I.
-Qed.
-
-Lemma sgvar_isptr:
-  forall i v rho, locald_denote (sgvar i v) rho -> isptr v.
-Proof.
-intros. hnf in H.
-destruct (Map.get (ge_of rho) i); try contradiction.
-subst; apply Coq.Init.Logic.I.
-Qed.
-
 Lemma lvar_eval_var:
  forall i t v rho, locald_denote (lvar i t v) rho -> eval_var i t rho = v.
 Proof.
@@ -392,6 +375,15 @@ Qed.
 
 Hint Extern 1 (isptr (eval_var _ _ _)) => (eapply lvar_isptr_eval_var; eassumption) : norm2.
 
+Lemma gvars_isptr:
+  forall Delta gv i rho t, tc_environ Delta rho -> (glob_types Delta) ! i = Some t -> locald_denote (gvars gv) rho -> isptr (gv i).
+Proof.
+intros. hnf in H1.
+subst.
+destruct_glob_types i.
+rewrite Heqo0.
+apply Coq.Init.Logic.I.
+Qed.
 
 Lemma force_val_sem_cast_neutral_isptr:
   forall v,
@@ -411,22 +403,15 @@ intros.
  apply lvar_isptr in H; destruct v; try contradiction; reflexivity.
 Qed.
 
-Lemma force_val_sem_cast_neutral_gvar:
-  forall i v rho,
-  locald_denote (gvar i v) rho ->
-  Some (force_val (sem_cast_pointer v)) = Some v.
+Lemma force_val_sem_cast_neutral_gvars:
+  forall Delta gv i t rho,
+  tc_environ Delta rho -> (glob_types Delta) ! i = Some t -> 
+  locald_denote (gvars gv) rho ->
+  Some (force_val (sem_cast_pointer (gv i))) = Some (gv i).
 Proof.
-intros.
- apply gvar_isptr in H; destruct v; try contradiction; reflexivity.
-Qed.
-
-Lemma force_val_sem_cast_neutral_sgvar:
-  forall i v rho,
-  locald_denote (sgvar i v) rho ->
-  Some (force_val (sem_cast_pointer v)) = Some v.
-Proof.
-intros.
- apply sgvar_isptr in H; destruct v; try contradiction; reflexivity.
+  intros.
+  eapply gvars_isptr in H; eauto.
+  destruct (gv i); try contradiction; reflexivity.
 Qed.
 
 Lemma prop_Forall_cons:
@@ -488,12 +473,11 @@ Ltac Forall_pTree_from_elements :=
    try autorewrite with entailer_rewrite in *;
    repeat first
    [ apply prop_Forall_cons1;
-     [unfold check_one_temp_spec, check_one_var_spec;
+     [unfold check_one_temp_spec, check_gvars_spec;
      simpl; auto;
      normalize;
      solve [eapply force_val_sem_cast_neutral_lvar; eassumption
-              | eapply force_val_sem_cast_neutral_gvar; eassumption
-              | eapply force_val_sem_cast_neutral_sgvar; eassumption
+              | eapply force_val_sem_cast_neutral_gvars; eassumption (* TODO: this line maybe problematic. -- by Qinxiang *)
               | apply force_val_sem_cast_neutral_isptr; auto
               ]
      | ]
@@ -502,7 +486,6 @@ Ltac Forall_pTree_from_elements :=
    | apply prop_Forall_nil'
    | apply prop_Forall_nil
    ];
- unfold check_one_temp_spec;
  simpl PTree.get.
 
 Lemma exp_uncurry2:
@@ -743,7 +726,6 @@ eapply (semax_call_id1_x_wow _ _ _ _ _ _ _ _ _ _ _ _ _ _ _ _ _ _ _ _ _ _ _ _ _ _
  | unfold fold_right_and; repeat rewrite and_True; auto
  ].
 
-
 Ltac forward_call_id1_y_wow :=
 let H := fresh in intro H;
 eapply (semax_call_id1_y_wow _ _ _ _ _ _ _ _ _ _ _ _ _ _ _ _ _ _ _ _ _ _ _ _ _ _ _ _ _ H); 
@@ -851,9 +833,6 @@ Ltac factor_out_v L :=
  match L with
  | temp _ ?v :: ?L' => factor_out_v' v L'
  | lvar _ _ ?v :: ?L' => factor_out_v' v L'
- | gvar _ ?v :: ?L' => factor_out_v' v L'
- | sgvar _ ?v :: ?L' => factor_out_v' v L'
- | localprop ?v ?L' => factor_out_v' v L'
  | _ => constr:(@nil val)
  end
  with factor_out_v' v L' := let x := fresh "v" in set (x:=v); 
@@ -2752,15 +2731,15 @@ Ltac solve_return_inner_gen :=
     end
  end.
 
-Inductive fn_data_at {cs: compspecs} (T2: PTree.t vardesc): ident * type -> mpred -> Prop :=
+Inductive fn_data_at {cs: compspecs} (Delta: tycontext) (T2: PTree.t (type * val)): ident * type -> mpred -> Prop :=
 | fn_data_at_intro: forall i t p,
     (complete_legal_cosu_type t && (sizeof t <? Int.modulus) && is_aligned cenv_cs ha_env_cs la_env_cs t 0 = true)%bool ->
-    msubst_eval_lvar T2 i t = Some p ->
-    fn_data_at T2 (i, t) (data_at_ Tsh t p).
+    msubst_eval_lvar Delta T2 i t = Some p ->
+    fn_data_at Delta T2 (i, t) (data_at_ Tsh t p).
 
-Lemma canonicalize_stackframe: forall {cs: compspecs} Delta P Q R T1 T2 G fn,
-  local2ptree Q = (T1, T2, nil, G) ->
-  Forall2 (fn_data_at T2) fn R ->
+Lemma canonicalize_stackframe: forall {cs: compspecs} Delta P Q R T1 T2 GV fn,
+  local2ptree Q = (T1, T2, nil, GV) ->
+  Forall2 (fn_data_at Delta T2) fn R ->
   local (tc_environ Delta) && PROPx P (LOCALx Q (SEPx R)) |-- fold_right sepcon emp (map (var_block Tsh) fn).
 Proof.
   intros.
@@ -2771,7 +2750,7 @@ Proof.
     apply (local2ptree_soundness P Q (y :: l')) in H; simpl app in H.
     inv H0.
     rewrite !andb_true_iff in H2; destruct H2 as [[? ?] ?].
-    apply (msubst_eval_lvar_eq P T1 T2 G (data_at_ Tsh t p :: l')) in H3.
+    apply (msubst_eval_lvar_eq Delta P T1 T2 GV (data_at_ Tsh t p :: l')) in H3.
     rewrite <- H in H3; clear H.
     rewrite (add_andp _ _ H3); clear H3.
     go_lowerx.
@@ -2786,7 +2765,7 @@ Proof.
   intros.
   go_lowerx.
 Qed.
-  
+
 Ltac solve_Forall2_fn_data_at :=
   solve
     [ apply Forall2_nil
@@ -3143,55 +3122,17 @@ subst; clear.
 simpl; f_equal. extensionality rho; normalize.
 Qed.
 
-Lemma intro_LOCAL_gvar:
-  forall Delta gv i P Q R,
-  (var_types Delta) ! i = None ->
-  (glob_types Delta) ! i <> None ->
-  In (gvars gv) Q ->
-  ENTAIL Delta, PROPx P (LOCALx Q (SEPx R)) |-- local (locald_denote (gvar i (gv i))).
-Proof.
-intros.
-Transparent andp.
-go_lowerx.
-Opaque andp.
-normalize.
-apply prop_right.
-pose proof (local_ext (locald_denote (gvars gv)) (map locald_denote Q) rho).
-apply H5 in H4.
-+
-simpl in H4.
-hnf.
-destruct_var_types i eqn:?H&?H.
-rewrite H7.
-destruct_glob_types i eqn:?H&?H; [| congruence].
-rewrite H4, H8.
-auto.
-+
-apply in_map.
-auto.
-Qed.
-
-Ltac assert_gvar i :=
- match goal with gv: globals |- context [gvars ?gv'] => constr_eq gv gv';
-   assert_LOCAL (gvar i (gv i)); 
-  [apply intro_LOCAL_gvar; 
-    [ reflexivity + fail 99  "Local variable " i " is shadowing the global variable" i
-    | (let H := fresh in intro H; discriminate H) + fail 99 "No global variable " i " in Delta, i.e., in your extern declarations"
-    | solve [repeat ((left; reflexivity) + right) ]] + fail 99 "No LOCAL assertion (gvars " gv ")"
-  | ]
- end.
-
 Ltac make_func_ptr id :=
- match goal with |- semax _ (PROPx _ (LOCALx ?Q _)) _ _ =>
-   lazymatch Q with context [gvar id _] => idtac | _ => assert_gvar id end
- end;
- eapply (make_func_ptr id); [reflexivity | reflexivity | reflexivity | reflexivity | ].
+  eapply (make_func_ptr id);
+  [ (reflexivity || fail 99  "Local variable " id " is shadowing the global variable" id)
+  | (reflexivity || fail 99 "No specification of function " id " in Delta")
+  | (reflexivity || fail 99 "No global variable " id " in Delta, i.e., in your extern declarations")
+  | split; reflexivity | ].
 
 Ltac change_mapsto_gvar_to_data_at :=
 match goal with gv: globals |- semax _ (PROPx _ (LOCALx ?L (SEPx ?S))) _ _ =>
   match S with
   | context [mapsto ?sh ?t (offset_val 0 (gv ?i)) ?v] =>
-      lazymatch L with context [gvar _ (gv i)] => idtac |  _ => assert_gvar i end;
       assert_PROP (headptr (offset_val 0 (gv i)));
           [entailer!;  apply <- headptr_offset_zero; auto |];
       erewrite (mapsto_data_at'' _ _ _ _ (offset_val _ (gv i)));
@@ -3199,7 +3140,6 @@ match goal with gv: globals |- semax _ (PROPx _ (LOCALx ?L (SEPx ?S))) _ _ =>
       match goal with H: _ |- _ => clear H end;
           rewrite <- ? data_at_offset_zero
   | context [mapsto ?sh ?t (gv ?i) ?v] =>
-      lazymatch L with context [gvar i (gv i)] => idtac |  _ => assert_gvar i end;
       assert_PROP (headptr (gv i));
           [entailer! |];
       erewrite (mapsto_data_at'' _ _ _ _ (gv i));
@@ -3304,7 +3244,6 @@ Fixpoint find_vars {A: Type} (f: ident -> A -> A) (e: expr) (x: A) : A :=
 Fixpoint find_lvars (locals: list localdef)  (m: PTree.t unit) : PTree.t unit :=
  match locals with
  | lvar i _ _ :: locals'=> find_lvars locals' (PTree.set i tt m)
- | gvar i _ :: locals'=> find_lvars locals' (PTree.set i tt m)
  | _ :: locals' => find_lvars locals' m
  | nil => m
  end.
@@ -3315,26 +3254,6 @@ Definition another_gvar (i: ident) (ml: PTree.t unit * list ident) : (PTree.t un
   match PTree.get i t with Some _ => ml | None =>  (PTree.set i tt t, i :: il) end
  end.
 Arguments another_gvar i !ml .
-
-Definition find_gvars (locals: list localdef) (c: statement) : list ident :=
- snd (find_expressions (find_vars another_gvar) c 
-                (find_lvars locals (PTree.empty _), nil)).
-
-Ltac assert_gvars' x := 
- match x with
- | ?i :: ?x' => assert_gvar i; assert_gvars' x'
- | nil => idtac
- end.
-
-Ltac assert_gvars := 
- match goal with |- semax _ (PROPx _ (LOCALx ?l _)) ?c _ =>
-   tryif match l with context [gvars _] => idtac end
-    then let x := constr:(find_gvars l c) in
-            let x := eval unfold find_gvars, find_lvars in x in
-            let x := eval simpl in x in 
-            assert_gvars' x
-   else idtac
- end.
 
 Ltac start_function_hint := idtac. (* "Hint: at any time, try the 'hint' tactic.  To disable this message, 'Ltac start_function_hint ::= idtac.' ". *)
 
@@ -3413,7 +3332,6 @@ Function spec: " S)
  | |- semax ?Delta (PROPx _ (LOCALx ?L _)) _ _ => check_parameter_vals Delta L
  | _ => idtac
  end;
- assert_gvars;
  clear_Delta_specs_if_leaf_function;
  start_function_hint.
 
